For every $x \in \AB^*$:
\begin{enumerate}[(i)]
    \item If $x \in \lang$ then there exists $c \in \AB^*$ such that $V$ accepts $(x, c)$.
    \item If $x \notin \lang$ then $V$ rejects $(x, c)$ for every $c \in \AB^*$.
    \item $V$ \textit{always} halts.
\end{enumerate}

We will show that $(0) \iff (b)$: \\

\underline{$(0) \Leftarrow (b)$}: \\
Let $V$ meet definition (b) for language $\lang$. $V$ also meets definition (0) for language $\lang$: \\
- (i) of (b) gives us directly (i) of (0). \\
- (ii) of (b) gives us directly (ii) of (0). \\
Hence we get $(0) \Leftarrow (b)$. \\

\underline{$(0) \Rightarrow (b)$}: \\
Let $V$ meet definition (0) for language $\lang$. \\
We saw in the recitation that $\exists V: V \text{ meets definition } (0) \text{ for } \lang \iff \lang \in \REcl$ \\
Therefore its enough to show that $\lang \in \REcl \Rightarrow \exists V: V \text{ meets definition } (b) \text{ for } \lang$  \\
Let $M$ be TM that accepts $\lang$. \\
We shall construct TM $V'$ that meets definition (b) for $\lang$. \\
$V'$ on input $(x, c)$:
\begin{enumerate}[1., itemsep=5pt]
    \item Run $M$ on input $x$ for $|c|$ steps.
    \item Accept if $M$ accepts.
    \item Reject.
\end{enumerate}

So we get: \\
If $x \in \lang$ \\
$\Longrightarrow \exists i \in \AB^*$ such that $M$ accepts $x$ (w.l.o.g.) after $i$ steps. \\
$\Longrightarrow \exists c_j \in \AB^*$ such that $M$ accepts $x$ after $|c_j|=i$ steps. \\
$\Longrightarrow \exists c_j \in \AB^*$ s.t. $V'$ accepts $(x, c_j)$. \\

If $x \notin \lang$ \\
$\Longrightarrow M$ does not accept $x$ after any amount of steps. \\
$\Longrightarrow V'$ rejects $(x, c)$ for every $c \in \AB^*$. \\

Also, notice that for every $(x, c)$, $V'$ will run $M$ for finite amount of steps and \\
then accept or reject, hence $V'$ halts for any input $(x, c)$. \\

Indeed, we get that $V'$ meets definition (b) for $\lang$. \\
So we get: \\
$\exists V: V \text{ meets definition } (0) \text{ for } \lang \Longrightarrow \lang \in \REcl \Longrightarrow \exists V: V \text{ meets definition } (b) \text{ for } \lang$ \\
Hence we get $(0) \Rightarrow (b)$. \\
