We need to show that: $w \in \lang \Longleftrightarrow  w \in \lang(D)$. \\
First we show that:
\[
    (*) \text{   } \hat{\de}([\empw], w) = \hat{\de}([\empw], w_1...w_k) = [\empw w_1...w_k] = [\empw w], \forall w =w_1...w_k \in \AB^*\\
\]
we will prove by induction on $k$ :

\underline{- Base Case:} \\
for $k=0$ we get: \\
\[
    w = w_1...w_k = \empw \rightarrow \hat{\de}([\empw], w) =  \hat{\de}([\empw], \empw) = [\empw] = [\empw w]
\] \\

\underline{- Induction Step}: \\
we will assume that the claim is correct for $w=w_1...w_k$ and prove for $w'=w_1...w_k \ch$ for $\ch \in \AB$:
\[
    \begin{aligned}
        \hat{\de}([\empw], w') & =                                                                                    \\
                               & = \hat{\de}([\empw], w_1...w_k\ch)        &  & (w'=w_1...w_k \ch)                    \\
                               & = \de(\hat{\de}([\empw], w_1...w_k), \ch) &  & (\text{from definition of }\hat{\de}) \\
                               & = \de([\empw w_1...w_k], \ch)             &  & (\text{from induction hypothesis})    \\
                               & = [\empw w_1...w_k \ch]                   &  & (\text{from definition of }\de)       \\
                               & = [\empw w']
    \end{aligned}
\]
Therefore by induction we get (*).

Now, we will prove $w \in \lang \Longleftrightarrow  w \in \lang(D)$: \\
Note that:
$ w = w_1...w_k \in \lang $

(from (*)) \\
$ \Longleftrightarrow \hat{\de}([\empw], w) = [\empw w] = [w] \subseteq \lang \text{ } (w \in \lang)$

(from previous section - section (a)) \\
$ \Longleftrightarrow \exists i \in \{0,...,n-1\}: \hat{\de}([\empw], w) = [w] = [x_i], [x_i] \in F $ \\

$ \Longleftrightarrow \hat{\de}(q_0, w) = \hat{\de}([\empw], w) \in F $ \\

$ \Longleftrightarrow  w \in \lang(D) $ \\
In conclusion, we got $w \in \lang \Longleftrightarrow  w \in \lang(D)$. Thus, concluding the proof. \\
